{"@context":{"rdf":"http://www.w3.org/1999/02/22-rdf-syntax-ns#","rdfs":"http://www.w3.org/2000/01/rdf-schema#","schema":"http://schema.org/","iot":"http://iotschema.org/"},"@graph":[{"@name":"iot:ChangeBinarySwitch","@type":"rdfs:Class","rdfs:subClassOf":"iot:ChangePropertyAction","rdfs:label":"ChangeBinarySwitch","rdfs:comment":"Specification of an action acting on some property of type BinarySwitch."},{"@name":"iot:ChangeCountDown","@type":"rdfs:Class","rdfs:subClassOf":"iot:ChangePropertyAction","rdfs:label":"ChangeCountDown","rdfs:comment":"Specification of an action acting on some property of type CountDown."},{"@name":"iot:ChangeCurrentColour","@type":"rdfs:Class","rdfs:subClassOf":"iot:ChangePropertyAction","rdfs:label":"ChangeCurrentColour","rdfs:comment":"Specification of an action acting on some property of type CurrentColour."},{"@name":"iot:ChangeCurrentDimmer","@type":"rdfs:Class","rdfs:subClassOf":"iot:ChangePropertyAction","rdfs:label":"ChangeCurrentDimmer","rdfs:comment":"Specification of an action acting on some property of type CurrentDimmer."},{"@name":"iot:ChangeCurrentLevel","@type":"rdfs:Class","rdfs:subClassOf":"iot:ChangePropertyAction","rdfs:label":"ChangeCurrentLevel","rdfs:comment":"Specification of an action acting on some property of type CurrentLevel."},{"@name":"iot:ChangeHumidity","@type":"rdfs:Class","rdfs:subClassOf":"iot:ChangePropertyAction","rdfs:label":"ChangeHumidity","rdfs:comment":"Specification of an action acting on some property of type Humidity."},{"@name":"iot:ChangeIlluminance","@type":"rdfs:Class","rdfs:subClassOf":"iot:ChangePropertyAction","rdfs:label":"ChangeIlluminance","rdfs:comment":"Specification of an action acting on some property of type Illuminance."},{"@name":"iot:ChangeMotionDetected","@type":"rdfs:Class","rdfs:subClassOf":"iot:ChangePropertyAction","rdfs:label":"ChangeMotionDetected","rdfs:comment":"Specification of an action acting on some property of type MotionDetected."},{"@name":"iot:ChangeMotionDetectedExt","@type":"rdfs:Class","rdfs:subClassOf":"iot:ChangePropertyAction","rdfs:label":"ChangeMotionDetectedExt","rdfs:comment":"Specification of an action acting on some property of type MotionDetectedExt."},{"@name":"iot:ChangeMotionType","@type":"rdfs:Class","rdfs:subClassOf":"iot:ChangePropertyAction","rdfs:label":"ChangeMotionType","rdfs:comment":"Specification of an action acting on some property of type MotionType."},{"@name":"iot:ChangeOperationStatus","@type":"rdfs:Class","rdfs:subClassOf":"iot:ChangePropertyAction","rdfs:label":"ChangeOperationStatus","rdfs:comment":"Specification of an action acting on some property of type OperationStatus."},{"@name":"iot:ChangeRampTime","@type":"rdfs:Class","rdfs:subClassOf":"iot:ChangePropertyAction","rdfs:label":"ChangeRampTime","rdfs:comment":"Specification of an action acting on some property of type RampTime."},{"@name":"iot:ChangeRunMode","@type":"rdfs:Class","rdfs:subClassOf":"iot:ChangePropertyAction","rdfs:label":"ChangeRunMode","rdfs:comment":"Specification of an action acting on some property of type RunMode."},{"@name":"iot:ChangeSetColour","@type":"rdfs:Class","rdfs:subClassOf":"iot:ChangePropertyAction","rdfs:label":"ChangeSetColour","rdfs:comment":"Specification of an action acting on some property of type SetColour."},{"@name":"iot:ChangeSetDimmer","@type":"rdfs:Class","rdfs:subClassOf":"iot:ChangePropertyAction","rdfs:label":"ChangeSetDimmer","rdfs:comment":"Specification of an action acting on some property of type SetDimmer."},{"@name":"iot:ChangeSwitchStatus","@type":"rdfs:Class","rdfs:subClassOf":"iot:ChangePropertyAction","rdfs:label":"ChangeSwitchStatus","rdfs:comment":"Specification of an action acting on some property of type SwitchStatus."},{"@name":"iot:ChangeTargetHumidity","@type":"rdfs:Class","rdfs:subClassOf":"iot:ChangePropertyAction","rdfs:label":"ChangeTargetHumidity","rdfs:comment":"Specification of an action acting on some property of type TargetHumidity."},{"@name":"iot:ChangeTargetTemperature","@type":"rdfs:Class","rdfs:subClassOf":"iot:ChangePropertyAction","rdfs:label":"ChangeTargetTemperature","rdfs:comment":"Specification of an action acting on some property of type TargetTemperature."},{"@name":"iot:ChangeTemperature","@type":"rdfs:Class","rdfs:subClassOf":"iot:ChangePropertyAction","rdfs:label":"ChangeTemperature","rdfs:comment":"Specification of an action acting on some property of type Temperature."},{"@name":"iot:ChangeTransitionTime","@type":"rdfs:Class","rdfs:subClassOf":"iot:ChangePropertyAction","rdfs:label":"ChangeTransitionTime","rdfs:comment":"Specification of an action acting on some property of type TransitionTime."},{"@name":"iot:ChangeTurnOff","@type":"rdfs:Class","rdfs:subClassOf":"iot:ChangePropertyAction","rdfs:label":"ChangeTurnOff","rdfs:comment":"Specification of an action acting on some property of type TurnOff."},{"@name":"iot:ChangeTurnOn","@type":"rdfs:Class","rdfs:subClassOf":"iot:ChangePropertyAction","rdfs:label":"ChangeTurnOn","rdfs:comment":"Specification of an action acting on some property of type TurnOn."},{"@name":"iot:ChangeWindStrength","@type":"rdfs:Class","rdfs:subClassOf":"iot:ChangePropertyAction","rdfs:label":"ChangeWindStrength","rdfs:comment":"Specification of an action acting on some property of type WindStrength."}]}