{
	"@context": {
		"rdf": "http://www.w3.org/1999/02/22-rdf-syntax-ns#",
		"rdfs": "http://www.w3.org/2000/01/rdf-schema#",
		"schema": "http://schema.org/",
		"iot": "http://iotschema.org/"
	},
	"@graph": [
		{
			"@id": "iot:ChangeBinarySwitch",
			"@type": "rdfs:Class",
			"rdfs:subClassOf": "iot:ChangePropertyAction",
			"rdfs:label": "ChangeBinarySwitch",
			"rdfs:comment": "Specification of an action acting on some property of type BinarySwitch."
		},
		{
			"@id": "iot:ChangeCountDown",
			"@type": "rdfs:Class",
			"rdfs:subClassOf": "iot:ChangePropertyAction",
			"rdfs:label": "ChangeCountDown",
			"rdfs:comment": "Specification of an action acting on some property of type CountDown."
		},
		{
			"@id": "iot:ChangeCurrentColour",
			"@type": "rdfs:Class",
			"rdfs:subClassOf": "iot:ChangePropertyAction",
			"rdfs:label": "ChangeCurrentColour",
			"rdfs:comment": "Specification of an action acting on some property of type CurrentColour."
		},
		{
			"@id": "iot:ChangeCurrentDimmer",
			"@type": "rdfs:Class",
			"rdfs:subClassOf": "iot:ChangePropertyAction",
			"rdfs:label": "ChangeCurrentDimmer",
			"rdfs:comment": "Specification of an action acting on some property of type CurrentDimmer."
		},
		{
			"@id": "iot:ChangeCurrentLevel",
			"@type": "rdfs:Class",
			"rdfs:subClassOf": "iot:ChangePropertyAction",
			"rdfs:label": "ChangeCurrentLevel",
			"rdfs:comment": "Specification of an action acting on some property of type CurrentLevel."
		},
		{
			"@id": "iot:ChangeHumidity",
			"@type": "rdfs:Class",
			"rdfs:subClassOf": "iot:ChangePropertyAction",
			"rdfs:label": "ChangeHumidity",
			"rdfs:comment": "Specification of an action acting on some property of type Humidity."
		},
		{
			"@id": "iot:ChangeIlluminance",
			"@type": "rdfs:Class",
			"rdfs:subClassOf": "iot:ChangePropertyAction",
			"rdfs:label": "ChangeIlluminance",
			"rdfs:comment": "Specification of an action acting on some property of type Illuminance."
		},
		{
			"@id": "iot:ChangeMotionDetected",
			"@type": "rdfs:Class",
			"rdfs:subClassOf": "iot:ChangePropertyAction",
			"rdfs:label": "ChangeMotionDetected",
			"rdfs:comment": "Specification of an action acting on some property of type MotionDetected."
		},
		{
			"@id": "iot:ChangeMotionDetectedExt",
			"@type": "rdfs:Class",
			"rdfs:subClassOf": "iot:ChangePropertyAction",
			"rdfs:label": "ChangeMotionDetectedExt",
			"rdfs:comment": "Specification of an action acting on some property of type MotionDetectedExt."
		},
		{
			"@id": "iot:ChangeMotionType",
			"@type": "rdfs:Class",
			"rdfs:subClassOf": "iot:ChangePropertyAction",
			"rdfs:label": "ChangeMotionType",
			"rdfs:comment": "Specification of an action acting on some property of type MotionType."
		},
		{
			"@id": "iot:ChangeOperationStatus",
			"@type": "rdfs:Class",
			"rdfs:subClassOf": "iot:ChangePropertyAction",
			"rdfs:label": "ChangeOperationStatus",
			"rdfs:comment": "Specification of an action acting on some property of type OperationStatus."
		},
		{
			"@id": "iot:ChangeRampTime",
			"@type": "rdfs:Class",
			"rdfs:subClassOf": "iot:ChangePropertyAction",
			"rdfs:label": "ChangeRampTime",
			"rdfs:comment": "Specification of an action acting on some property of type RampTime."
		},
		{
			"@id": "iot:ChangeRunMode",
			"@type": "rdfs:Class",
			"rdfs:subClassOf": "iot:ChangePropertyAction",
			"rdfs:label": "ChangeRunMode",
			"rdfs:comment": "Specification of an action acting on some property of type RunMode."
		},
		{
			"@id": "iot:ChangeSetColour",
			"@type": "rdfs:Class",
			"rdfs:subClassOf": "iot:ChangePropertyAction",
			"rdfs:label": "ChangeSetColour",
			"rdfs:comment": "Specification of an action acting on some property of type SetColour."
		},
		{
			"@id": "iot:ChangeSetDimmer",
			"@type": "rdfs:Class",
			"rdfs:subClassOf": "iot:ChangePropertyAction",
			"rdfs:label": "ChangeSetDimmer",
			"rdfs:comment": "Specification of an action acting on some property of type SetDimmer."
		},
		{
			"@id": "iot:ChangeSwitchStatus",
			"@type": "rdfs:Class",
			"rdfs:subClassOf": "iot:ChangePropertyAction",
			"rdfs:label": "ChangeSwitchStatus",
			"rdfs:comment": "Specification of an action acting on some property of type SwitchStatus."
		},
		{
			"@id": "iot:ChangeTargetHumidity",
			"@type": "rdfs:Class",
			"rdfs:subClassOf": "iot:ChangePropertyAction",
			"rdfs:label": "ChangeTargetHumidity",
			"rdfs:comment": "Specification of an action acting on some property of type TargetHumidity."
		},
		{
			"@id": "iot:ChangeTargetTemperature",
			"@type": "rdfs:Class",
			"rdfs:subClassOf": "iot:ChangePropertyAction",
			"rdfs:label": "ChangeTargetTemperature",
			"rdfs:comment": "Specification of an action acting on some property of type TargetTemperature."
		},
		{
			"@id": "iot:ChangeTemperature",
			"@type": "rdfs:Class",
			"rdfs:subClassOf": "iot:ChangePropertyAction",
			"rdfs:label": "ChangeTemperature",
			"rdfs:comment": "Specification of an action acting on some property of type Temperature."
		},
		{
			"@id": "iot:ChangeTransitionTime",
			"@type": "rdfs:Class",
			"rdfs:subClassOf": "iot:ChangePropertyAction",
			"rdfs:label": "ChangeTransitionTime",
			"rdfs:comment": "Specification of an action acting on some property of type TransitionTime."
		},
		{
			"@id": "iot:ChangeTurnOff",
			"@type": "rdfs:Class",
			"rdfs:subClassOf": "iot:ChangePropertyAction",
			"rdfs:label": "ChangeTurnOff",
			"rdfs:comment": "Specification of an action acting on some property of type TurnOff."
		},
		{
			"@id": "iot:ChangeTurnOn",
			"@type": "rdfs:Class",
			"rdfs:subClassOf": "iot:ChangePropertyAction",
			"rdfs:label": "ChangeTurnOn",
			"rdfs:comment": "Specification of an action acting on some property of type TurnOn."
		},
		{
			"@id": "iot:ChangeWindStrength",
			"@type": "rdfs:Class",
			"rdfs:subClassOf": "iot:ChangePropertyAction",
			"rdfs:label": "ChangeWindStrength",
			"rdfs:comment": "Specification of an action acting on some property of type WindStrength."
		}
	]
}