{
	"@context": {
		"rdf": "http://www.w3.org/1999/02/22-rdf-syntax-ns#",
		"rdfs": "http://www.w3.org/2000/01/rdf-schema#",
		"schema": "http://schema.org/",
		"iot": "http://iotschema.org/"
	},
	"@graph": [
		{
			"@id": "iot:BinarySwitchChanged",
			"@type": "rdfs:Class",
			"rdfs:subClassOf": "iot:PropertyChangedEvent",
			"rdfs:label": "BinarySwitchChanged",
			"rdfs:comment": "Specification of an event occurring when some property of type BinarySwitch changes."
		},
		{
			"@id": "iot:CountDownChanged",
			"@type": "rdfs:Class",
			"rdfs:subClassOf": "iot:PropertyChangedEvent",
			"rdfs:label": "CountDownChanged",
			"rdfs:comment": "Specification of an event occurring when some property of type CountDown changes."
		},
		{
			"@id": "iot:CurrentColourChanged",
			"@type": "rdfs:Class",
			"rdfs:subClassOf": "iot:PropertyChangedEvent",
			"rdfs:label": "CurrentColourChanged",
			"rdfs:comment": "Specification of an event occurring when some property of type CurrentColour changes."
		},
		{
			"@id": "iot:CurrentDimmerChanged",
			"@type": "rdfs:Class",
			"rdfs:subClassOf": "iot:PropertyChangedEvent",
			"rdfs:label": "CurrentDimmerChanged",
			"rdfs:comment": "Specification of an event occurring when some property of type CurrentDimmer changes."
		},
		{
			"@id": "iot:CurrentLevelChanged",
			"@type": "rdfs:Class",
			"rdfs:subClassOf": "iot:PropertyChangedEvent",
			"rdfs:label": "CurrentLevelChanged",
			"rdfs:comment": "Specification of an event occurring when some property of type CurrentLevel changes."
		},
		{
			"@id": "iot:HumidityChanged",
			"@type": "rdfs:Class",
			"rdfs:subClassOf": "iot:PropertyChangedEvent",
			"rdfs:label": "HumidityChanged",
			"rdfs:comment": "Specification of an event occurring when some property of type Humidity changes."
		},
		{
			"@id": "iot:IlluminanceChanged",
			"@type": "rdfs:Class",
			"rdfs:subClassOf": "iot:PropertyChangedEvent",
			"rdfs:label": "IlluminanceChanged",
			"rdfs:comment": "Specification of an event occurring when some property of type Illuminance changes."
		},
		{
			"@id": "iot:MotionDetectedChanged",
			"@type": "rdfs:Class",
			"rdfs:subClassOf": "iot:PropertyChangedEvent",
			"rdfs:label": "MotionDetectedChanged",
			"rdfs:comment": "Specification of an event occurring when some property of type MotionDetected changes."
		},
		{
			"@id": "iot:MotionDetectedExtChanged",
			"@type": "rdfs:Class",
			"rdfs:subClassOf": "iot:PropertyChangedEvent",
			"rdfs:label": "MotionDetectedExtChanged",
			"rdfs:comment": "Specification of an event occurring when some property of type MotionDetectedExt changes."
		},
		{
			"@id": "iot:MotionTypeChanged",
			"@type": "rdfs:Class",
			"rdfs:subClassOf": "iot:PropertyChangedEvent",
			"rdfs:label": "MotionTypeChanged",
			"rdfs:comment": "Specification of an event occurring when some property of type MotionType changes."
		},
		{
			"@id": "iot:OperationStatusChanged",
			"@type": "rdfs:Class",
			"rdfs:subClassOf": "iot:PropertyChangedEvent",
			"rdfs:label": "OperationStatusChanged",
			"rdfs:comment": "Specification of an event occurring when some property of type OperationStatus changes."
		},
		{
			"@id": "iot:RampTimeChanged",
			"@type": "rdfs:Class",
			"rdfs:subClassOf": "iot:PropertyChangedEvent",
			"rdfs:label": "RampTimeChanged",
			"rdfs:comment": "Specification of an event occurring when some property of type RampTime changes."
		},
		{
			"@id": "iot:RunModeChanged",
			"@type": "rdfs:Class",
			"rdfs:subClassOf": "iot:PropertyChangedEvent",
			"rdfs:label": "RunModeChanged",
			"rdfs:comment": "Specification of an event occurring when some property of type RunMode changes."
		},
		{
			"@id": "iot:SetColourChanged",
			"@type": "rdfs:Class",
			"rdfs:subClassOf": "iot:PropertyChangedEvent",
			"rdfs:label": "SetColourChanged",
			"rdfs:comment": "Specification of an event occurring when some property of type SetColour changes."
		},
		{
			"@id": "iot:SetDimmerChanged",
			"@type": "rdfs:Class",
			"rdfs:subClassOf": "iot:PropertyChangedEvent",
			"rdfs:label": "SetDimmerChanged",
			"rdfs:comment": "Specification of an event occurring when some property of type SetDimmer changes."
		},
		{
			"@id": "iot:SwitchStatusChanged",
			"@type": "rdfs:Class",
			"rdfs:subClassOf": "iot:PropertyChangedEvent",
			"rdfs:label": "SwitchStatusChanged",
			"rdfs:comment": "Specification of an event occurring when some property of type SwitchStatus changes."
		},
		{
			"@id": "iot:TargetHumidityChanged",
			"@type": "rdfs:Class",
			"rdfs:subClassOf": "iot:PropertyChangedEvent",
			"rdfs:label": "TargetHumidityChanged",
			"rdfs:comment": "Specification of an event occurring when some property of type TargetHumidity changes."
		},
		{
			"@id": "iot:TargetTemperatureChanged",
			"@type": "rdfs:Class",
			"rdfs:subClassOf": "iot:PropertyChangedEvent",
			"rdfs:label": "TargetTemperatureChanged",
			"rdfs:comment": "Specification of an event occurring when some property of type TargetTemperature changes."
		},
		{
			"@id": "iot:TemperatureChanged",
			"@type": "rdfs:Class",
			"rdfs:subClassOf": "iot:PropertyChangedEvent",
			"rdfs:label": "TemperatureChanged",
			"rdfs:comment": "Specification of an event occurring when some property of type Temperature changes."
		},
		{
			"@id": "iot:TransitionTimeChanged",
			"@type": "rdfs:Class",
			"rdfs:subClassOf": "iot:PropertyChangedEvent",
			"rdfs:label": "TransitionTimeChanged",
			"rdfs:comment": "Specification of an event occurring when some property of type TransitionTime changes."
		},
		{
			"@id": "iot:TurnOffChanged",
			"@type": "rdfs:Class",
			"rdfs:subClassOf": "iot:PropertyChangedEvent",
			"rdfs:label": "TurnOffChanged",
			"rdfs:comment": "Specification of an event occurring when some property of type TurnOff changes."
		},
		{
			"@id": "iot:TurnOnChanged",
			"@type": "rdfs:Class",
			"rdfs:subClassOf": "iot:PropertyChangedEvent",
			"rdfs:label": "TurnOnChanged",
			"rdfs:comment": "Specification of an event occurring when some property of type TurnOn changes."
		},
		{
			"@id": "iot:WindStrengthChanged",
			"@type": "rdfs:Class",
			"rdfs:subClassOf": "iot:PropertyChangedEvent",
			"rdfs:label": "WindStrengthChanged",
			"rdfs:comment": "Specification of an event occurring when some property of type WindStrength changes."
		}
	]
}